

Solutions

(01)

$$x^2 + 2x - 4 = 0$$

$$\therefore \alpha + \beta = -\frac{b}{a} = \frac{-2}{1} = -2$$

$$\alpha\beta = \frac{c}{a} = \frac{-4}{1} = -4$$

$$\alpha^2 + \beta^2 = (\alpha + \beta)^2 - 2\alpha\beta$$

$$= (-2)^2 - 2(-4)$$

$$= 4 + 8$$

$$= 12$$

$$\alpha^4 + \beta^4 = (\alpha^2 + \beta^2)^2 - 2\alpha^2\beta^2$$

$$= (12)^2 - 2(-4)^2$$

$$= 144 - 32$$

$$= 112$$

$$\text{let } A = \alpha^4 + \frac{1}{\beta^2}$$

$$B = \beta^4 + \frac{1}{\alpha^2}$$

$$\begin{aligned}
 A+B &= \left(\alpha^4 + \frac{1}{\beta^2} \right) + \left(\beta^4 + \frac{1}{\alpha^2} \right) \quad (02) \\
 &= \left(\alpha^4 + \beta^4 \right) + \left(\frac{1}{\alpha^2} + \frac{1}{\beta^2} \right) \\
 &= \left(\alpha^4 + \beta^4 \right) + \frac{(\alpha^2 + \beta^2)}{(\alpha\beta)^2}
 \end{aligned}$$

$$= 112 + \frac{12}{(-4)^2}$$

$$= 112 + \frac{3}{4}$$

$$= \frac{451}{4}$$

$$AB = \left(\alpha^4 + \frac{1}{\beta^2} \right) \left(\beta^4 + \frac{1}{\alpha^2} \right)$$

$$= \alpha^4 \beta^4 + (\alpha^2 + \beta^2) + \frac{1}{\alpha^2 \beta^2}$$

$$= (-4)^4 + 12 + \frac{1}{(-4)^2}$$

$$= 256 + 12 + \frac{1}{16}$$

$$= \frac{4289}{16}$$

$$\therefore x^2 - \frac{451}{4}x + \frac{4289}{16} = 0$$

$$(02) \quad x^2 - 4\sqrt{2} kx + 2k^4 - 1 = 0$$

$$\alpha^2 + \beta^2 = 66$$

$$\alpha + \beta = -\frac{b}{a} = 4\sqrt{2}k$$

$$\alpha\beta = \frac{c}{a} = 2k^4 - 1$$

$$(\alpha + \beta)^2 = \alpha^2 + \beta^2 + 2\alpha\beta$$

$$(4\sqrt{2}k)^2 = 66 + 2(2k^4 - 1)$$

$$32k^2 = 66 + 2(2k^4 - 1)$$

$$16k^2 = 33 + 2k^4 - 1$$

$$2k^4 - 16k^2 + 32 = 0$$

$$k^4 - 8k^2 + 16 = 0$$

$$(k^2 - 4)^2 = 0$$

$$k^2 = 4$$

$$k = 2 \quad (\because k > 0)$$

(03)

$$(\alpha + \beta)^3 = \alpha^3 + 3\alpha^2\beta + 3\alpha\beta^2 + \beta^3 \quad (04)$$

$$(4\sqrt{2}k)^3 = \alpha^3 + \beta^3 + 3\alpha\beta(\alpha + \beta)$$

$$(8\sqrt{2})^3 = \alpha^3 + \beta^3 + 3(2k^4 - 1)(4\sqrt{2}k)$$

$$(8\sqrt{2})^3 = \alpha^3 + \beta^3 + 3 \times 31 \times 8\sqrt{2}$$

$$1024\sqrt{2} = \alpha^3 + \beta^3 + 744\sqrt{2}$$

$$\therefore \alpha^3 + \beta^3 = 280\sqrt{2}$$

$$(06) \quad x^3 - 6x^2 + 4x + 12 = 0$$

$$\alpha + \beta + \gamma = -\frac{b}{a} = -\frac{(-6)}{1} = 6$$

$$\alpha\beta + \beta\gamma + \gamma\alpha = \frac{c}{a} = \frac{4}{1} = 4$$

$$\alpha\beta\gamma = -\frac{d}{a} = -\frac{12}{1} = -12$$

$$(a) \therefore \alpha + \beta + \gamma = 6$$

$$(b) (\alpha + \beta + \gamma)^2 = \alpha^2 + \beta^2 + \gamma^2 + 2\alpha\beta + 2\beta\gamma + 2\gamma\alpha$$

$$\begin{aligned} \alpha^2 + \beta^2 + \gamma^2 &= (\alpha + \beta + \gamma)^2 - 2(\alpha\beta + \beta\gamma + \gamma\alpha) \\ &= 6^2 - 2 \times 4 \\ &= 28 \end{aligned}$$

$$\begin{aligned} (c) \quad \frac{1}{\alpha} + \frac{1}{\beta} + \frac{1}{\gamma} &= \frac{\beta\gamma + \alpha\gamma + \alpha\beta}{\alpha\beta\gamma} \\ &= \frac{4}{-12} \\ &= -\frac{1}{3} \end{aligned}$$

(08) Let the roots be $\alpha, 2\alpha, 4\alpha$

(06)

$$\therefore \alpha + 2\alpha + 4\alpha = -\frac{b}{a}$$

$$\therefore 7\alpha = -\frac{b}{a} \quad \text{--- (1)}$$

$$2\alpha^2 + 8\alpha^2 + 4\alpha^2 = \frac{c}{a}$$

$$\therefore 14\alpha^2 = \frac{c}{a} \quad \text{--- (2)}$$

$$8\alpha^3 = -\frac{d}{a} \quad \text{--- (3)}$$

$$\textcircled{1} \times \textcircled{2} \Rightarrow$$

$$7 \times 14 \alpha^3 = -\frac{b}{a} \times \frac{c}{a}$$

$$98\alpha^3 = -\frac{bc}{a^2} \quad \text{--- (4)}$$

$$\textcircled{4} / \textcircled{3} \Rightarrow$$

$$\frac{98\alpha^3}{8\alpha^3} = -\frac{bc}{a^2} \times -\frac{a}{d}$$

$$\frac{49}{4} = \frac{bc}{ad}$$

$$49ad = 4bc$$